

1. Written : Understanding Word2Vec

(a) $y_w = \begin{cases} 1 & (w=0) \\ 0 & (w \neq 0) \end{cases}$

$$-\sum_{w \in \text{Vocab}} y_w \log \hat{y}_w = -y_0 \log \hat{y}_0 - \sum_{w \neq 0} y_w \log \hat{y}_w = -\log \hat{y}_0$$

$$\mathcal{J}_{\text{naive-softmax}} = -\log \frac{\exp(u_0^T v_c)}{\sum_{w \in \text{Vocab}} \exp(u_w^T v_c)} = -\log \hat{y}_0$$

(b) $\frac{\partial \mathcal{J}_{\text{naive-softmax}}}{\partial v_c} = \frac{\partial}{\partial v_c} \left(-\log \frac{\exp(u_0^T v_c)}{\sum_{w \in \text{Vocab}} \exp(u_w^T v_c)} \right) = \frac{\partial}{\partial v_c} \left(-\log \exp(u_0^T v_c) + \log \sum_{w \in \text{Vocab}} \exp(u_w^T v_c) \right)$

$$= -\frac{1}{\exp(u_0^T v_c)} \cdot \exp(u_0^T v_c) \cdot u_0 + \frac{1}{\sum_{w \in \text{Vocab}} \exp(u_w^T v_c)} \cdot \left(\sum_{w \in \text{Vocab}} \exp(u_w^T v_c) \cdot u_w \right)$$

$$= -u_0 + \frac{\sum_{w \in \text{Vocab}} \exp(u_w^T v_c)}{\sum_{w \in \text{Vocab}} \exp(u_w^T v_c)} \cdot u_w = -u_0 + \sum_{w \in \text{Vocab}} \hat{y}_w \cdot u_w$$

$$= -y_0 u_0 + \sum_{w \in \text{Vocab}} \hat{y}_w u_w = \sum_{w \in \text{Vocab}} -y_w \cdot u_w + \hat{y}_w \cdot u_w$$

$$= \sum_{w \in \text{Vocab}} (\hat{y}_w - y_w) \cdot u_w \quad \begin{matrix} \text{scalar} & \text{vector (dx)} \end{matrix} \quad \left\{ \begin{array}{l} u = [u_1, u_2, \dots, u_0, \dots, u_{|\text{Vocab}|}] \in \mathbb{R}^{d \times |\text{Vocab}|} \\ y \in \mathbb{R}^{|\text{Vocab}| \times 1}, \hat{y} \in \mathbb{R}^{|\text{Vocab}| \times 1} \end{array} \right.$$

$$\therefore \frac{\partial \mathcal{J}_{\text{naive-softmax}}}{\partial v_c} = u \cdot (\hat{y} - y)$$

(c) $\frac{\partial \mathcal{J}_{\text{naive-softmax}}}{\partial u_w} = \frac{\partial}{\partial u_w} \left(-\log \left(\frac{\exp(u_0^T v_c)}{\sum_{w \in \text{Vocab}} \exp(u_w^T v_c)} \right) \right) = \frac{\partial}{\partial u_w} (-u_0^T v_c + \log \sum_{w \in \text{Vocab}} \exp(u_w^T v_c))$

i) $w=0$

$$\frac{\partial}{\partial u_w} (-u_0^T v_c + \log \sum_{w \in \text{Vocab}} \exp(u_w^T v_c)) = -v_c + \frac{\exp(u_0^T v_c)}{\sum_{w \in \text{Vocab}} \exp(u_w^T v_c)} \cdot v_c = -v_c + \hat{y}_0 \cdot v_c = (\hat{y}_0 - 1) \cdot v_c$$

ii) $w \neq 0$

$$\frac{\partial}{\partial u_w} (-u_0^T v_c + \log \sum_{w \in \text{Vocab}} \exp(u_w^T v_c)) = 0 + \frac{\exp(u_w^T v_c)}{\sum_{w \in \text{Vocab}} \exp(u_w^T v_c)} \cdot v_c = \hat{y}_w \cdot v_c$$

$$\therefore \frac{\partial \mathcal{J}_{\text{naive-softmax}}}{\partial u_w} = (\hat{y}_w - y_w) v_c \quad \begin{cases} (\hat{y}_0 - 1) \cdot v_c & (w=0) \\ \hat{y}_w \cdot v_c & (w \neq 0) \end{cases}$$

(d) $\frac{\partial \mathcal{J}_{\text{naive-softmax}}}{\partial u} = \left[\frac{\partial \mathcal{J}}{\partial u_1}, \frac{\partial \mathcal{J}}{\partial u_2}, \dots, \frac{\partial \mathcal{J}}{\partial u_{|\text{Vocab}|}} \right] = [(\hat{y}_1 - y_1) \cdot v_c, (\hat{y}_2 - y_2) \cdot v_c, \dots, (\hat{y}_{|\text{Vocab}|} - y_{|\text{Vocab}|}) \cdot v_c]$

$$= v_c \cdot (\hat{y} - y)^T$$

(e) $\mathcal{J}_{\text{neg}}(v_c, 0, u) = -\log \sigma(u_0^T v_c) - \sum_{s=1}^K \log \sigma(-u_{w_s}^T v_c)$

(i) $\frac{\partial}{\partial x} \sigma(x) = \frac{\partial}{\partial x} \left(\frac{1}{e^{-x} + 1} \right) = e^{-x} \cdot \frac{1}{(e^{-x} + 1)^2} = \frac{1}{e^{-x} + 1} \cdot \left(1 - \frac{1}{e^{-x} + 1} \right) = \sigma(x) \cdot (1 - \sigma(x))$

$$\frac{\partial \mathcal{J}}{\partial v_c} = -\frac{1}{\sigma(u_0^T v_c)} \cdot \sigma(u_0^T v_c) \cdot (1 - \sigma(u_0^T v_c)) \cdot u_0 - \sum_{s=1}^K \frac{1}{\sigma(-u_{w_s}^T v_c)} \cdot \sigma(-u_{w_s}^T v_c) \cdot (1 - \sigma(-u_{w_s}^T v_c)) \cdot (-u_{w_s})$$

$$= (\sigma(u_0^T v_c) - 1) \cdot u_0 + \sum_{s=1}^K (1 - \sigma(-u_{w_s}^T v_c)) \cdot u_{w_s} = (\sigma(u_0^T v_c) - 1) \cdot u_0 + \sum_{s=1}^K \sigma(u_{w_s}^T v_c) \cdot u_{w_s}$$

$$(\because 1 - \sigma(-x)) = 1 - \frac{1}{1 + e^x} = \frac{e^x}{1 + e^x} = \frac{1}{e^{-x} + 1} = \sigma(x)$$

$$\frac{\partial \mathcal{J}}{\partial u_0} = -\frac{1}{\sigma(u_0^T v_c)} \cdot \sigma(u_0^T v_c) \cdot (1 - \sigma(u_0^T v_c)) \cdot v_c = (\sigma(u_0^T v_c) - 1) \cdot v_c$$

$$\frac{\partial \mathcal{J}}{\partial u_{w_s}} = -\frac{1}{\sigma(-u_{w_s}^T v_c)} \cdot (1 - \sigma(-u_{w_s}^T v_c)) \cdot (-v_c) = \sigma(u_{w_s}^T v_c) \cdot v_c$$

$$\therefore \begin{cases} \frac{\partial \mathcal{J}}{\partial v_c} = (\sigma(u_0^T v_c) - 1) \cdot u_0 + \sum_{s=1}^K \sigma(u_{w_s}^T v_c) \cdot u_{w_s} \\ \frac{\partial \mathcal{J}}{\partial u_0} = (\sigma(u_0^T v_c) - 1) \cdot v_c \\ \frac{\partial \mathcal{J}}{\partial u_{w_s}} = \sigma(u_{w_s}^T v_c) \cdot v_c \end{cases}$$

(ii) Negative sampling only computes K terms, which is much smaller than total vocabulary.

(f) (i) $\frac{\partial \mathcal{J}_{\text{skip}}}{\partial u} = -\sum_{u \leq j \leq u, j \neq 0} \frac{\partial \mathcal{J}(v_c, w_{t+j}, u)}{\partial u}$

(ii) $\frac{\partial \mathcal{J}_{\text{skip}}}{\partial v_c} = -\sum_{u \leq j \leq u, j \neq 0} \frac{\partial \mathcal{J}(v_c, w_{t+j}, u)}{\partial v_c}$

(iii) $\frac{\partial \mathcal{J}_{\text{skip}}}{\partial v_w} (w \neq c) = 0$ (No term of $v_w \rightarrow$ Derivatives will be zero.)